Add reference implementation of `prune_updates` (#246)
### Description:

A detailed description of your contribution. Why is this change
necessary?

### Testing:

What tests have been run? Did `make all` succeed for your changes? Was
conformance testing successful on an Aarch64 machine?

### License:

By submitting this pull request, I confirm that my contribution is
made under the terms of the Apache 2.0 license.

---------

Co-authored-by: Siddharth <siddu.druid@gmail.com>

Tactics/BvOmegaBench.lean
@@ -60,10 +60,10 @@ def run (g : MVarId) (hyps : Array Expr) (bvToNatSimpCtx : Simp.Context) (bvToNa
      /- Wow, this is gross. I need to filter out the fvars, and keep track of which ones I use for simplification. -/
      try
        let (result?, _stats) ← g.withContext <| simpGoal g bvToNatSimpCtx bvToNatSimprocs (simplifyTarget := true) (discharge? := .none) hypFVars
-       let .some (hypFVars', g') := result? | return ()
+       let .some (_hypFVars', g') := result? | return ()
        g := g'
        let hypsOldRetained ← g.withContext <| pure (← getLCtx).getFVarIds
-       let hypsOldRetained := hypsOldRetained.filter (fun fvar => hypFVars.contains fvar)
+       let _hypsOldRetained := hypsOldRetained.filter (fun fvar => hypFVars.contains fvar)
        -- hypFVars := hypFVars'
      catch e => 
        trace[simp_mem.info] "in BvOmega, ran `simp only [bv_toNat]` and got error: {indentD e.toMessageData}"
