Proofs/AES-GCM/GCMGmultV8Sym.lean
@@ -134,31 +134,80 @@ multiplication into four constituent ones, for normalization.
 example :
   let p := 0b11#2
   let q := 0b10#2
-  let w := 0b01#2
-  let z := 0b01#2
+  let x := 0b01#2
+  let y := 0b01#2
   (DPSFP.polynomial_mult
         (p ++ q)
-        (w ++ z))
+        (x ++ y))
   =
-  ((DPSFP.polynomial_mult p w) ++ 0#4) ^^^
-  (0#4 ++ (DPSFP.polynomial_mult q z)) ^^^
-  (0#2 ++ (DPSFP.polynomial_mult p z) ++ 0#2) ^^^
-  (0#2 ++ (DPSFP.polynomial_mult q w) ++ 0#2) := by native_decide
+  ((DPSFP.polynomial_mult p x) ++ 0#4) ^^^
+  (0#4 ++ (DPSFP.polynomial_mult q y)) ^^^
+  (0#2 ++ (DPSFP.polynomial_mult p y) ++ 0#2) ^^^
+  (0#2 ++ (DPSFP.polynomial_mult q x) ++ 0#2) := by native_decide
 
+def pmult_test_1 : IO Bool := do
+  let p ← BitVec.rand 64
+  let q ← BitVec.rand 64
+  let x ← BitVec.rand 64
+  let y ← BitVec.rand 64
+  pure
+    (DPSFP.polynomial_mult (p ++ q) (x ++ y) ==
+     ((DPSFP.polynomial_mult p x) ++ 0#128) ^^^
+     (0#128 ++ (DPSFP.polynomial_mult q y)) ^^^
+     (0#64 ++ (DPSFP.polynomial_mult p y) ++ 0#64) ^^^
+     (0#64 ++ (DPSFP.polynomial_mult q x) ++ 0#64))
 
+/--
+info: true
+-/
+#guard_msgs in
+#eval pmult_test_1
+
+theorem DPSFP.polynomial_mult_append {p q x y : BitVec 64} :
+  DPSFP.polynomial_mult (p ++ q) (x ++ y) =
+  ((DPSFP.polynomial_mult p x) ++ 0#128) ^^^
+   (0#128 ++ (DPSFP.polynomial_mult q y)) ^^^
+   (0#64 ++ (DPSFP.polynomial_mult p y) ++ 0#64) ^^^
+   (0#64 ++ (DPSFP.polynomial_mult q x) ++ 0#64) := by
+  sorry
+
+/-
+Source: Function `GCMInitV8` in `Specs/GCMV8.lean`:
+Note that `H0` is the 128-bit HTable input to `gcm_gmult_v8`.
+
+let H2 := GCMV8.gcm_polyval H0 H0
+let H1 := ((hi H2) ^^^ (lo H2)) ++ ((hi H0) ^^^ (lo H0))
+-/
+
+set_option maxRecDepth 8000 in
+set_option maxHeartbeats 500000 in
 set_option pp.deepTerms false in
 set_option pp.deepTerms.threshold 50 in
 -- set_option trace.simp_mem.info true in
 #time theorem gcm_gmult_v8_program_run_27 (s0 sf : ArmState)
+    {H1_hi H1_lo H0_hi H0_lo : BitVec 64}
     (h_s0_program : s0.program = gcm_gmult_v8_program)
     (h_s0_err : read_err s0 = .None)
     (h_s0_pc : read_pc s0 = gcm_gmult_v8_program.min)
     (h_s0_sp_aligned : CheckSPAlignment s0)
     (h_Xi : Xi = s0[read_gpr 64 0#5 s0, 16])
-    (h_HTable : HTable = s0[read_gpr 64 1#5 s0, 32])
+    (h_HTable_lo : H0_hi ++ H0_lo = s0[read_gpr 64 1#5 s0, 16])
+    (h_HTable_hi : H1_hi ++ H1_lo = s0[read_gpr 64 1#5 s0 + 16#64, 16])
+    -- (h_HTable : HTable = s0[read_gpr 64 1#5 s0, 32])
+    -- (h_HTable_alt : HTable = H1_hi ++ H1_lo ++ H0_hi ++ H0_lo)
+    (h_H1_low_64 : H1_lo = H0_hi ^^^ H0_lo)
+    -- (h_H1 : HTable.extractLsb' 128 128 =
+    --         let H0 := HTable.extractLsb' 0 128
+    --         let H2 := GCMV8.gcm_polyval H0 H0
+    --         let H0_hi := H0.extractLsb' 64 64
+    --         let H0_lo := H0.extractLsb' 0 64
+    --         let H2_hi := H2.extractLsb' 64 64
+    --         let H2_lo := H2.extractLsb' 0 64
+    --         ((H2_hi) ^^^ (H2_lo)) ++ ((H0_hi) ^^^ (H0_lo)))
     (h_mem_sep : Memory.Region.pairwiseSeparate
                  [(read_gpr 64 0#5 s0, 16),
-                  (read_gpr 64 1#5 s0, 32)])
+                  (read_gpr 64 1#5 s0, 16),
+                  (read_gpr 64 1#5 s0 + 16#64, 16)])
     (h_run : sf = run gcm_gmult_v8_program.length s0) :
     -- The final state is error-free.
     read_err sf = .None ∧
@@ -168,11 +217,6 @@ set_option pp.deepTerms.threshold 50 in
     CheckSPAlignment sf ∧
     -- The final state returns to the address in register `x30` in `s0`.
     read_pc sf = r (StateField.GPR 30#5) s0 ∧
-    -- (TODO) Delete the following conjunct because it is covered by the
-    -- MEM_UNCHANGED_EXCEPT frame condition. We keep it around because it
-    -- exposes the issue with `simp_mem` that @bollu will fix.
-    -- HTable is unmodified.
-    sf[read_gpr 64 1#5 s0, 32] = HTable ∧
     -- Frame conditions.
     -- Note that the following also covers that the Xi address in .GPR 0
     -- is unmodified.
@@ -185,24 +229,24 @@ set_option pp.deepTerms.threshold 50 in
     sf[r (.GPR 0) s0, 16] =
     rev_elems 128 8
             (GCMV8.GCMGmultV8_alt
-              (HTable.extractLsb' 0 128)
+              (H0_hi ++ H0_lo)
               (rev_elems 128 8 Xi (by decide) (by decide)))
             (by decide) (by decide) := by
   -- Prelude
   simp_all only [state_simp_rules, -h_run]
-  simp only [Nat.reduceMul] at Xi HTable
+  -- simp only [Nat.reduceMul] at Xi HTable
+  simp only [Nat.reduceMul] at Xi
   simp (config := {ground := true}) only at h_s0_pc
   -- ^^ Still needed, because `gcm_gmult_v8_program.min` is somehow
   --    unable to be reflected
-
   sym_n 27
   -- Epilogue
-  simp only [←Memory.mem_eq_iff_read_mem_bytes_eq] at *
+  -- simp only [←Memory.mem_eq_iff_read_mem_bytes_eq] at *
   simp only [memory_rules] at *
   sym_aggregate
   -- Split conjunction
   repeat' apply And.intro
-  · simp_mem; rfl
+  -- · simp_mem; rfl
   · simp only [List.mem_cons, List.mem_singleton, not_or, and_imp] at *
     sym_aggregate
   · intro n addr h_separate
@@ -211,27 +255,9 @@ set_option pp.deepTerms.threshold 50 in
       simp_mem sep with [h_separate]
   · clear_named [h_s, stepi_]
     clear s1 s2 s3 s4 s5 s6 s7 s8 s9 s10 s11 s12 s13 s14 s15 s16 s17 s18 s19 s20 s21 s22 s23 s24 s25 s26
+
     -- Simplifying the LHS
-    have h_HTable_low :
-      Memory.read_bytes 16 (r (StateField.GPR 1#5) s0) s0.mem = HTable.extractLsb' 0 128 := by
-      -- (FIXME @bollu) use `simp_mem` instead of the rw below.
-      -- conv => 
-      --   lhs
-      --   simp_mem sub r 
-      rw [@Memory.read_bytes_eq_extractLsBytes_sub_of_mem_subset'
-           32 (r (StateField.GPR 1#5) s0) HTable (r (StateField.GPR 1#5) s0) 16 _ h_HTable.symm]
-      · simp only [Nat.reduceMul, BitVec.extractLsBytes, Nat.sub_self, Nat.zero_mul]
-      · mem_omega!
-    have h_HTable_high :
-      (Memory.read_bytes 16 (r (StateField.GPR 1#5) s0 + 16#64) s0.mem) = HTable.extractLsb' 128 128 := by
-      -- (FIXME @bollu) use `simp_mem` instead of the rw below.
-      -- conv => 
-      --   lhs
-      --   simp_mem sub r 
-      rw [@Memory.read_bytes_eq_extractLsBytes_sub_of_mem_subset'
-          32 (r (StateField.GPR 1#5) s0) HTable (r (StateField.GPR 1#5) s0 + 16#64) 16 _ h_HTable.symm]
-      repeat sorry
-    simp only [h_HTable_high, h_HTable_low, ←h_Xi]
+    simp only [←h_Xi]
     clear h_mem_sep h_run
     /-
     simp/ground below to reduce
@@ -251,11 +277,12 @@ set_option pp.deepTerms.threshold 50 in
     rw [@vrev128_64_8_in_terms_of_rev_elems (by decide) (by decide) (by decide) (by decide)] at h_Xi_rev
     generalize h_Xi_upper_rev : rev_elems 64 8 (BitVec.extractLsb' 64 64 Xi) (by decide) (by decide) = Xi_upper_rev
     generalize h_Xi_lower_rev : rev_elems 64 8 (BitVec.extractLsb' 0 64 Xi) (by decide) (by decide) = Xi_lower_rev
-    -- Simplifying the RHS
+
     simp only [GCMV8.GCMGmultV8_alt,
                GCMV8.lo, GCMV8.hi,
                GCMV8.gcm_polyval,
-               ←h_HTable, ←h_Xi_rev, h_Xi_lower_rev, h_Xi_upper_rev]
+               ←h_HTable_lo, ←h_HTable_hi,
+               ←h_Xi_rev, h_Xi_lower_rev, h_Xi_upper_rev]
     simp only [pmull_op_e_0_eize_64_elements_1_size_128_eq, gcm_polyval_mul_eq_polynomial_mult]
     simp only [zeroExtend_allOnes_lsh_64, zeroExtend_allOnes_lsh_0]
     rw [BitVec.extractLsb'_64_128_of_appends]
@@ -265,20 +292,7 @@ set_option pp.deepTerms.threshold 50 in
     repeat rw [BitVec.extractLsb'_zero_extractLsb'_of_le (by decide)]
     repeat rw [BitVec.extractLsb'_extractLsb'_zero_of_le (by decide)]
     rw [BitVec.and_high_to_extractLsb'_concat]
-    generalize h_HTable_upper : (BitVec.extractLsb' 64 64 HTable) = HTable_upper
-    generalize h_HTable_lower : (BitVec.extractLsb' 0 64 HTable) = HTable_lower
-    generalize h_term_u0u1 : (DPSFP.polynomial_mult HTable_upper Xi_upper_rev) = u0u1 at *
-    generalize h_term_l0l1 : (DPSFP.polynomial_mult HTable_lower Xi_lower_rev) = l0l1 at *
-    generalize h_term_1 : (DPSFP.polynomial_mult (BitVec.extractLsb' 128 64 HTable) (Xi_lower_rev ^^^ Xi_upper_rev) ^^^
-                        BitVec.extractLsb' 64 128 (l0l1 ++ u0u1) ^^^
-                      (u0u1 ^^^ l0l1)) = term_1
-    generalize h_term_2 : ((term_1 &&& 0xffffffffffffffff#128 ||| BitVec.zeroExtend 128 (BitVec.setWidth 64 u0u1) <<< 64) ^^^
-                  DPSFP.polynomial_mult (BitVec.extractLsb' 0 64 u0u1) 0xc200000000000000#64)
-                  = term_2
-    generalize h_term_3 : (BitVec.extractLsb' 64 128 (term_2 ++ term_2) ^^^
-            (BitVec.extractLsb' 64 64 l0l1 ++ 0x0#64 |||
-              BitVec.zeroExtend 128 (BitVec.extractLsb' 64 64 term_1) <<< 0))
-              = term_3
+
     rw [@vrev128_64_8_in_terms_of_rev_elems (by decide) (by decide) (by decide) (by decide)]
     rw [BitVec.extractLsb'_64_128_of_appends]
     rw [@rev_elems_64_8_append_eq_rev_elems_128_8 _ _ (by decide) (by decide) (by decide) (by decide)]
@@ -286,11 +300,28 @@ set_option pp.deepTerms.threshold 50 in
     rw [@rev_elems_128_8_eq_rev_elems_64_8_extractLsb' _ (by decide) (by decide) (by decide) (by decide) (by decide)]
     rw [h_Xi_upper_rev, h_Xi_lower_rev]
     rw [BitVec.extractLsb'_append_eq]
-    simp [GCMV8.gcm_polyval_red]
-    -- have h_reduce : (GCMV8.reduce 0x100000000000000000000000000000087#129 0x1#129) = 1#129 := by native_decide
-    -- simp [GCMV8.gcm_polyval_red, GCMV8.irrepoly, GCMV8.pmod, h_reduce]
-    -- repeat (unfold GCMV8.pmod.pmodTR; simp)
+    simp only [BitVec.truncate_eq_setWidth, Nat.reduceAdd, BitVec.shiftLeft_zero_eq]
 
+    simp [DPSFP.polynomial_mult_append]
+    simp [GCMV8.gcm_polyval_red, GCMV8.irrepoly]
+
+    generalize h_term_1 : DPSFP.polynomial_mult H0_lo Xi_lower_rev = term1
+    generalize h_term_2 : DPSFP.polynomial_mult H0_hi Xi_upper_rev = term2
+
+    -- (TODO) Can we remove `reverse` from `pmod` in the RHS?
+
+    -- have h_reduce : (GCMV8.reduce 0x100000000000000000000000000000087#129 0x1#129) = 1#129 := by native_decide
+    --
+    -- simp only [GCMV8.gcm_polyval_red, GCMV8.irrepoly,
+    --            GCMV8.pmod, GCMV8.pmod.pmodTR,
+    --            GCMV8.reduce, GCMV8.degree, GCMV8.degree.degreeTR]
+    -- simp only [Nat.reduceAdd, BitVec.ushiftRight_eq, BitVec.reduceExtracLsb',
+    --   BitVec.reduceHShiftLeft, BitVec.reduceAppend, BitVec.reduceHShiftRight, BitVec.ofNat_eq_ofNat,
+    --   BitVec.reduceEq, ↓reduceIte, Nat.sub_self, BitVec.ushiftRight_zero_eq, BitVec.reduceAnd,
+    --   BitVec.toNat_ofNat, Nat.pow_one, Nat.reduceMod, Nat.mul_zero, Nat.add_zero, Nat.zero_mod,
+    --   Nat.zero_add, Nat.sub_zero, Nat.mul_one, Nat.zero_mul, Nat.one_mul, Nat.reduceSub,
+    --   BitVec.and_self, BitVec.zero_and, BitVec.reduceMul, BitVec.xor_zero, BitVec.mul_one,
+    --   BitVec.zero_xor, Nat.add_one_sub_one, BitVec.one_mul, BitVec.reduceXOr]
     sorry
   done
 
