Tactics/PruneUpdatesLogic.lean
@@ -1,0 +1,612 @@
+/-
+Copyright (c) 2024 Amazon.com, Inc. or its affiliates. All Rights Reserved.
+Released under Apache 2.0 license as described in the file LICENSE.
+Author(s): Shilpi Goel
+-/
+
+/-
+Experimental method to aggregate state effects using reflection.
+
+In LNSym, we already have a language that describes writes to the `ArmState`
+using functions `w`. However, these writes can shadow others, which causes the
+nest of writes to grow large. We reflect `w` and to get a pruned nest of writes.
+As a simple example, consider the following nest of writes:
+```
+s1 = w .PC pc (w (.GPR 0) x0 (w .PC pc' (w (.GPR 0) x0' s0)))
+```
+We would like to prune this to the equivalent term below:
+```
+s1 = w .PC pc (w (.GPR 0) x0 s0)
+```
+
+Note that we do not reflect memory updates at this point.
+
+This is inspired by `simp_arith`, especially the following files:
+
+`[lean] Init/Data/Nat/Linear.lean`
+`[lean] Meta/Tactic/LinearAith/Nat/Basic.lean`
+`[lean] Meta/Tactic/LinearAith/Nat/Simp.lean`
+-/
+
+import Arm.Exec
+import Arm.FromMathlib
+
+namespace ArmConstr
+
+/- We use `Nat`s to refer to all the variables in our context. -/
+abbrev StateVar  := Nat
+abbrev GPRVar    := Nat
+abbrev SFPVar    := Nat
+abbrev PCVar     := Nat
+abbrev ErrVar    := Nat
+abbrev FlagVar   := Nat
+
+inductive Var where
+  | state (var : StateVar)
+  | gpr   (var : GPRVar)
+  | sfp   (var : SFPVar)
+  | pc    (var : PCVar)
+  | err   (var : ErrVar)
+  | flag  (var : FlagVar)
+  deriving Repr, DecidableEq, Inhabited
+
+abbrev StateContext := List ArmState
+abbrev GPRContext   := List (BitVec 64)
+abbrev SFPContext   := List (BitVec 128)
+abbrev PCContext    := List (BitVec 64)
+abbrev FlagContext  := List (BitVec 1)
+abbrev ErrContext  := List (StateError)
+
+/--
+Context containing all the variables encountered in the problem. The
+position of a variable in the context becomes variable name (see, e.g.,
+`StateVar`, which is a `Nat`).
+-/
+structure Context where
+  state : StateContext
+  err   : ErrContext
+  pc    : PCContext
+  gpr   : GPRContext
+  sfp   : SFPContext
+  flag  : FlagContext
+  deriving Repr, Inhabited
+
+def Val (var : Var) : Type :=
+  match var with
+  | .state _ => ArmState
+  | .gpr _ => BitVec 64
+  | .sfp _ => BitVec 128
+  | .pc _ => BitVec 64
+  | .flag _ => BitVec 1
+  | .err _ => StateError
+
+/--
+Look up variable `v` in the `StateContext`.
+-/
+def StateVar.denote (ctx : StateContext) (v : StateVar) : ArmState :=
+  ctx.getD v ArmState.default
+
+/--
+Look up variable `v` in the `GPRContext`.
+-/
+def GPRVar.denote (ctx : GPRContext) (v : GPRVar) : BitVec 64 :=
+  ctx.getD v 0
+
+@[local simp]
+theorem GPRVar.denote_of_var :
+  GPRVar.denote ctx v = ctx.getD v 0 := by
+  simp [GPRVar.denote]
+
+/--
+Look up variable `v` in the `SFPContext`.
+-/
+def SFPVar.denote (ctx : SFPContext) (v : SFPVar) : BitVec 128 :=
+  ctx.getD v 0
+
+/--
+Look up variable `v` in the `PCContext`.
+-/
+def PCVar.denote (ctx : PCContext) (v : PCVar) : BitVec 64 :=
+  ctx.getD v 0
+
+/--
+Look up variable `v` in the `ErrContext`.
+-/
+def ErrVar.denote (ctx : ErrContext) (v : ErrVar) : StateError :=
+  ctx.getD v StateError.None
+
+/--
+Look up variable `v` in the `FlagContext`.
+-/
+def FlagVar.denote (ctx : FlagContext) (v : FlagVar) : BitVec 1 :=
+  ctx.getD v 0
+
+/--
+Look up `var` in the appropriate field of `ctx`, indicated by `fld`.
+-/
+def Var.denote (ctx : Context) (fld : StateField) (var : Nat) : state_value fld :=
+  match fld with
+  | .GPR _   => GPRVar.denote ctx.gpr var
+  | .SFP _   => SFPVar.denote ctx.sfp var
+  | .PC      => PCVar.denote ctx.pc var
+  | .FLAG _  => FlagVar.denote ctx.flag var
+  | .ERR     => ErrVar.denote ctx.err var
+
+/--
+Datastructure that characterizes all the updates that can be made to an
+`ArmState`.
+-/
+inductive Update where
+  | err  (v : ErrVar)
+  | pc   (v : PCVar)
+  | gpr  (i : BitVec 5) (v : GPRVar)
+  | sfp  (i : BitVec 5) (v : SFPVar)
+  | flag (i : PFlag)    (v : FlagVar)
+ deriving DecidableEq, Repr, Inhabited
+
+instance : ToString Update where toString a := toString (repr a)
+
+instance : Lean.ToMessageData Update where
+  toMessageData x := match x with
+  | .err v    => m!"(err {v})"
+  | .pc v     => m!"(pc {v})"
+  | .gpr i v  => m!"(gpr {i} {v})"
+  | .sfp i v  => m!"(sfp {i} {v})"
+  | .flag i v => m!"(flag {i} {v})"
+
+abbrev Updates := List Update
+
+/--
+`StateField` characterized by the `Update u`.
+-/
+def Update.field (u : Update) : StateField :=
+  match u with
+  | .err _ => StateField.ERR
+  | .pc _ => StateField.PC
+  | .gpr i _ => StateField.GPR i
+  | .sfp i _ => StateField.SFP i
+  | .flag i _ => StateField.FLAG i
+
+/--
+Variable ensconsed in `Update u`.
+-/
+def Update.var (u : Update) : Nat :=
+  match u with
+  | Update.err v    => v
+  | Update.pc v     => v
+  | Update.gpr _ v  => v
+  | Update.sfp _ v  => v
+  | Update.flag _ v => v
+
+/--
+Do updates `x` and `y` refer to the same state component?
+-/
+def Update.regEq (x y : Update) : Prop :=
+  match x, y with
+  | err _, err _ => True
+  | pc _, pc _ => True
+  | gpr i _, gpr j _ => i = j
+  | sfp i _, sfp j _ => i = j
+  | flag i _, flag j _ => i = j
+  | _, _ => False
+
+-- set_option diagnostics true in
+-- instance : Decidable (Update.regEq x y) :=
+--   inferInstanceAs (Decidable <|
+--     match x, y with
+--     | .pc _, .pc _ => True
+--     | .gpr i _, .gpr j _ => i = j
+--     | .sfp i _, .sfp j _ => i = j
+--     | .flag i _, .flag j _ => i = j
+--     | _, _ => False)
+
+private def PFlag.natIdx (f : PFlag) : Nat :=
+  match f with
+  | .N => 0
+  | .Z => 1
+  | .C => 2
+  | .V => 3
+
+/--
+Is the field of update `x` "less than or equal to" that of `y`?
+-/
+def Update.regIndexLe (x y : Update) : Bool :=
+  match x, y with
+  | err _, _ => true
+  | _, err _ => false
+  | pc _, _ => true
+  | _, pc _ => false
+  | gpr i _, gpr j _ => i <= j
+  | gpr _ _, _ => true
+  | _, gpr _ _ => false
+  | sfp i _, sfp j _ => i <= j
+  | sfp _ _, _ => true
+  | _, sfp _ _ => false
+  | flag i _, flag j _ => PFlag.natIdx i <= PFlag.natIdx j
+
+theorem Update.regIndexLe_trans (a b c : Update)
+  (h1 : Update.regIndexLe a b)
+  (h2 : Update.regIndexLe b c) :
+  Update.regIndexLe a c := by
+  simp_all [Update.regIndexLe]
+  cases a <;> cases b <;> cases c <;> simp_all
+  repeat (exact BitVec.le_trans h1 h2)
+  exact Nat.le_trans h1 h2
+  done
+
+theorem Update.regIndexLe_total (a b : Update) :
+  Update.regIndexLe a b || Update.regIndexLe b a := by
+  simp [Update.regIndexLe]
+  cases a <;> cases b <;> simp_all
+  repeat apply BitVec.le_total
+  apply Nat.le_total
+  done
+
+/--
+Datastructure to represent expressions characterizing the following state
+update.
+```
+curr_state = writes[prev_state]
+```
+-/
+structure Expr where
+   curr_state : StateVar
+   prev_state : StateVar
+   writes : Updates
+deriving DecidableEq, Repr, Inhabited
+
+/--
+Map updates `us` to state `prev_state` to an `ArmState`.
+-/
+def Expr.denote_writes (ctx : Context) (us : Updates) (prev_state : StateVar)
+  : ArmState :=
+  match us with
+  | [] => StateVar.denote ctx.state prev_state
+  | Update.gpr i v :: rest =>
+    w (.GPR i)
+      (GPRVar.denote ctx.gpr v)
+      (Expr.denote_writes ctx rest prev_state)
+  | Update.sfp i v :: rest =>
+    w (.SFP i)
+      (SFPVar.denote ctx.sfp v)
+      (Expr.denote_writes ctx rest prev_state)
+  | Update.pc v :: rest =>
+    w .PC
+      (PCVar.denote ctx.pc v)
+      (Expr.denote_writes ctx rest prev_state)
+  | Update.err v :: rest =>
+    w .ERR
+      (ErrVar.denote ctx.err v)
+      (Expr.denote_writes ctx rest prev_state)
+  | Update.flag i v :: rest =>
+    w (.FLAG i)
+      (FlagVar.denote ctx.flag v)
+      (Expr.denote_writes ctx rest prev_state)
+
+@[local simp]
+theorem denote_writes_empty :
+  Expr.denote_writes ctx [] prev_state = StateVar.denote ctx.state prev_state := by
+  simp only [Expr.denote_writes]
+
+@[local simp]
+theorem denote_writes_cons :
+  Expr.denote_writes ctx (e :: us) prev_state =
+  w (Update.field e) (Var.denote ctx (Update.field e) (Update.var e))
+    (Expr.denote_writes ctx us prev_state) := by
+  conv => lhs; unfold Expr.denote_writes
+  simp_all [Update.field, Update.var, Var.denote]
+  split
+  · -- Empty updates
+    simp_all
+  · -- GPR update
+    rename_i heq i' v i h_cons
+    have h_cons_1 : e = Update.gpr i' v := by simp_all
+    have h_cons_2 : us = i := by simp_all
+    rw [h_cons_1]; simp_all
+  · -- SFP update
+    rename_i heq i' v i h_cons
+    have h_cons_1 : e = Update.sfp i' v := by simp_all
+    have h_cons_2 : us = i := by simp_all
+    rw [h_cons_1]; simp_all
+  · -- PC update
+    rename_i heq i' v i
+    have h_cons_1 : e = Update.pc i' := by simp_all
+    have h_cons_2 : us = v := by simp_all
+    rw [h_cons_1]; simp_all
+  · -- ERR update
+    rename_i heq i' v i
+    have h_cons_1 : e = Update.err i' := by simp_all
+    have h_cons_2 : us = v := by simp_all
+    rw [h_cons_1]; simp_all
+  · -- Flag update
+    rename_i heq i' v i h_cons
+    have h_cons_1 : e = Update.flag i' v := by simp_all
+    have h_cons_2 : us = i := by simp_all
+    rw [h_cons_1]; simp_all
+  done
+
+theorem denote_statevar_eq_denote_writes_eq
+  (h : StateVar.denote ctx.state v1 = StateVar.denote ctx.state v2) :
+  Expr.denote_writes ctx writes v1 = Expr.denote_writes ctx writes v2 := by
+  induction writes
+  case nil => simpa [Expr.denote_writes]
+  case cons =>
+    rename_i head tail h_ind
+    simp [Expr.denote_writes]
+    simp_all only
+  done
+
+private theorem denote_writes_sorted_helper
+  (h : ∀ (b : Update), b ∈ l1 → (!head.regIndexLe b) = true) :
+  Expr.denote_writes ctx (l1 ++ head :: l2) s =
+  Expr.denote_writes ctx (head :: l1 ++ l2) s := by
+  induction l1
+  case nil => simp_all only [List.not_mem_nil,
+                             Bool.not_eq_eq_eq_not,
+                             Bool.not_true, false_implies,
+                             implies_true, List.nil_append,
+                             denote_writes_cons,
+                             List.singleton_append]
+  case cons =>
+    rename_i head' tail' ih
+    simp [denote_writes_cons]
+    rw [ih]
+    simp only [List.cons_append, denote_writes_cons]
+    · rw [w_of_w_commute]
+      simp_all [Update.regIndexLe, Update.field]
+      obtain ⟨h1, h2⟩ := h
+      clear h2
+      cases head <;> try simp_all <;> cases head' <;>
+      try simp_all <;> try exact BitVec.ne_of_lt h1
+      rename_i i1 _ i2 _
+      cases i1 <;> cases i2 <;> try simp_all
+    · simp_all
+
+/--
+Sorting `Updates xs` using `Update.regIndexLe` is immaterial to their denotation
+over `StateVar s`. This is because sorting preserves the order of shadowed
+updates in `xs`, which means that the most recent one appears first in the
+sorted list (see `w_of_w_shadow`); changing the order of independent updates
+does not affect the semantics (see, e.g., `w_of_w_commute`).
+-/
+@[local simp]
+theorem denote_writes_sorted :
+  Expr.denote_writes ctx (List.mergeSort xs Update.regIndexLe) s =
+  Expr.denote_writes ctx xs s := by
+  induction xs
+  case nil => simp only [List.mergeSort_nil, denote_writes_empty]
+  case cons =>
+    rename_i head tail ih
+    simp only [denote_writes_cons]
+    have ⟨l1, l2, h1, h2, h3⟩ :=
+      @List.mergeSort_cons Update Update.regIndexLe
+        (by apply Update.regIndexLe_trans)
+        (by apply Update.regIndexLe_total)
+        head tail
+    rw [h1]
+    simp_all only [Bool.not_eq_eq_eq_not,
+                   Bool.not_true,
+                   denote_writes_sorted_helper h3,
+                   List.cons_append, denote_writes_cons]
+    done
+
+
+/--
+Denote an `Expr e` to a `Prop` corresponding to `curr_state = writes[prev_state]`.
+-/
+def Expr.denote (ctx : Context) (e : Expr) : Prop :=
+  StateVar.denote ctx.state e.curr_state =
+  Expr.denote_writes ctx e.writes e.prev_state
+
+/--
+Return a `Prop` corresponding to `e1 = e2`.
+-/
+def Expr.denote_eq (ctx : Context) (e1 e2 : Expr) : Prop :=
+  StateVar.denote ctx.state e1.prev_state = StateVar.denote ctx.state e2.prev_state ∧
+  StateVar.denote ctx.state e1.curr_state = StateVar.denote ctx.state e2.curr_state ∧
+  Expr.denote ctx e1 ∧
+  Expr.denote ctx e2
+
+abbrev Exprs := List Expr
+
+/--
+Denote each expression in `es` using `Expr.denote`.
+-/
+def Exprs.denote (ctx : Context) (es : Exprs) : Prop :=
+  -- es.foldl (init := True) (fun p e => p ∧ e.denote ctx)
+  match es with
+  | [] => True
+  | u :: rest => Expr.denote ctx u ∧ Exprs.denote ctx rest
+
+def Expr.default : Expr :=
+  { prev_state := 0, curr_state := 0, writes := [] }
+
+open Expr Update in
+/--
+info: true
+-/
+#guard_msgs in
+#eval List.mergeSort [.gpr 1#5 1, .gpr 1#5 2] Update.regIndexLe =
+      -- If a write shadows another, then `List.mergeSort` with `Update.regIndexLe`
+      -- will preserve the order of the writes.
+      [.gpr 1#5 1, .gpr 1#5 2]
+
+/--
+Erase repeated adjacent elements. Keeps the first occurrence of each run.
+
+Non tail-recursive version.
+-/
+def Expr.eraseReps (us : Updates) : Updates :=
+  match us with
+  | [] => []
+  | [x] => [x]
+  | x :: y :: rest =>
+    match x.field == y.field with
+    | true => eraseReps (x :: rest)
+    | false => x :: eraseReps (y :: rest)
+
+@[local simp]
+theorem denote_writes_eraseReps :
+  Expr.denote_writes ctx (Expr.eraseReps xs) s =
+  Expr.denote_writes ctx xs s := by
+  induction xs using Expr.eraseReps.induct
+  case case1 =>
+    simp_all [Expr.eraseReps]
+  case case2 =>
+    rename_i x
+    simp [Expr.eraseReps]
+  case case3 =>
+    rename_i x y rest h_eq ih
+    simp [Expr.eraseReps, h_eq]
+    simp [Update.field] at h_eq
+    cases x <;> try simp_all <;> cases y <;>
+    try simp_all [Update.field, Update.var] <;>
+    rw [h_eq, w_of_w_shadow]
+    all_goals (simp_all [Update.field, Update.var]; rw [w_of_w_shadow])
+  case case4 =>
+    rename_i x y rest h_eq ih
+    simp [Expr.eraseReps, h_eq]
+    simp [Update.field] at h_eq
+    simp_all
+    done
+
+def Expr.eraseAdjReps.loop (u : Update) (us rs : Updates) : Updates :=
+match u, us, rs with
+| a, [], rs => (a::rs).reverse
+| a, a'::as, rs =>
+  match a.field == a'.field with
+  | true  => loop a as rs
+  | false => loop a' as (a::rs)
+
+/--
+Tail-recursive version of `Expr.eraseReps`.
+
+(FIXME) Prove equivalent to `Expr.eraseReps`.
+-/
+def Expr.eraseAdjReps (us : Updates) : Updates :=
+  match us with
+  | []    => []
+  | a::as => Expr.eraseAdjReps.loop a as []
+
+@[local simp]
+theorem Expr.eraseAdjReps_empty :
+  eraseAdjReps [] = [] := by
+  simp [eraseAdjReps]
+
+@[local simp]
+theorem Expr.eraseAdjReps_one :
+  eraseAdjReps [a] = [a] := by
+  simp [eraseAdjReps]
+  unfold eraseAdjReps.loop; simp
+
+private theorem Expr.eraseAdjReps.loop_eq :
+  Expr.eraseAdjReps.loop x (u :: us) rs =
+  if x.field == u.field then Expr.eraseAdjReps.loop x us rs
+                        else Expr.eraseAdjReps.loop u us (x :: rs) := by
+  simp [loop]
+  split
+  · rename_i h_eq
+    simp_all [Update.field]
+  · rename_i h_eq
+    simp_all [Update.field]
+  done
+
+private theorem Expr.eraseAdjReps.loop_append :
+  Expr.eraseAdjReps.loop x xs (acc2 ++ acc1) =
+  acc1.reverse ++ (Expr.eraseAdjReps.loop x xs acc2) := by
+  induction xs generalizing x acc1 acc2
+  case nil => simp [Expr.eraseAdjReps.loop]
+  case cons =>
+    rename_i head tail ih
+    simp [Expr.eraseAdjReps.loop]
+    split
+    · rename_i h_eq
+      simp [Update.field] at h_eq
+      rw [ih]
+    · rename_i h_neq
+      simp [Update.field] at h_neq
+      have : (x :: (acc2 ++ acc1)) = x :: acc2 ++ acc1 := by
+        simp only [List.cons_append]
+      rw [this, ih]
+      done
+
+-- #check Expr.eraseReps.induct
+-- #check Expr.eraseAdjReps.loop.induct
+/-
+theorem Expr.eraseReps_and_eraseAdjReps.loop :
+  acc.reverse ++ eraseReps (x :: xs) = eraseAdjReps.loop x xs acc := by
+  induction x, xs, acc using eraseAdjReps.loop.induct
+  case case1 => simp [eraseAdjReps.loop, eraseReps]
+  case case2 =>
+    rename_i a a' as rs h_eq ih
+    simp [eraseReps, eraseAdjReps.loop, h_eq]
+    sorry
+  repeat sorry
+-/
+
+def Expr.prune (e : Expr) : Expr :=
+  let e_sorted := List.mergeSort e.writes Update.regIndexLe
+  let e_nodups := eraseReps e_sorted
+  { e with writes := e_nodups }
+
+open Expr Update in
+/--
+info: { curr_state := 1,
+  prev_state := 0,
+  writes := [ArmConstr.Update.pc 0,
+             ArmConstr.Update.sfp 0x00#5 3,
+             ArmConstr.Update.sfp 0x01#5 2,
+             ArmConstr.Update.sfp 0x02#5 1,
+             ArmConstr.Update.sfp 0x03#5 0] }
+-/
+#guard_msgs in
+#eval Expr.prune { curr_state := 1,
+                   prev_state := 0,
+                   writes := [(.pc 0),
+                              (.sfp 0x03#5 0),
+                              (.pc 1),
+                              (.sfp 0x02#5 1),
+                              (.pc 2),
+                              (.sfp 0x01#5 2),
+                              (.pc 3),
+                              (.sfp 0x00#5 3)]}
+
+/--
+Does removing shadowed writes in `e1` give `e2`?
+-/
+def Expr.isPruned (e1 e2 : Expr) : Bool :=
+  prune e1 == e2
+
+theorem Expr.eq_true_of_denote (ctx : Context) (e1 e2 : Expr) :
+  (Expr.isPruned e1 e2) → Expr.denote ctx e1 → Expr.denote ctx e2 := by
+  simp [isPruned, prune, denote]
+  intro h; cases e2
+  rename_i s1 s0 writes; simp_all only [mk.injEq]
+  rw [←h.right.right]; clear h
+  simp only [denote_writes_eraseReps, denote_writes_sorted, implies_true]
+  done
+
+#time
+open Expr Update in
+theorem example1
+  (h_s1 : s1 = w (.GPR 0#5) x0 (w (.GPR 1#5) x1 (w (.GPR 0#5) x1 s0))) :
+  s1 = w (.GPR 0#5) x0 (w (.GPR 1#5) x1 s0) := by
+  exact
+    ((Expr.eq_true_of_denote { state := [s0, s1],
+                               gpr := [x0, x1],
+                               sfp := [],
+                               pc := [],
+                               flag := [],
+                               err := [] }
+        -- e1
+        { prev_state := 0, curr_state := 1,
+          writes := [.gpr 0#5 (0), .gpr 1#5 (1), .gpr 0#5 (1)] }
+        -- e2
+        { prev_state := 0, curr_state := 1,
+          writes := [.gpr 0#5 (0), .gpr 1#5 (1)] }
+        (by native_decide)))
+    h_s1
+
+-- #print example1
+
+end ArmConstr
