Tactics/SymBlock.lean
@@ -1,0 +1,247 @@
+/-
+Copyright (c) 2024 Amazon.com, Inc. or its affiliates. All Rights Reserved.
+Released under Apache 2.0 license as described in the file LICENSE.
+Author(s): Shilpi Goel, Alex Keizer
+-/
+import Arm.Exec
+import Arm.Memory.MemoryProofs
+import Tactics.FetchAndDecode
+import Tactics.Sym.Context
+import Tactics.Sym
+
+import Lean
+
+open BitVec
+open Lean
+open Lean.Meta Lean.Elab.Tactic
+
+open AxEffects SymContext
+open Sym (withTraceNode withInfoTraceNode traceHeartbeats)
+
+/-- `init_next_block h_run blocki_eq sn block_size steps_left` splits the hypothesis
+  `h_run: s_final = run (n + block_size) s`
+by adding a new state variable, `sn`, and two new hypotheses:
+  `blocki_eq : run block_size s = s_next`
+  `h_run'   : s_final = run n s_next`
+to the local context of the main goal.
+The names are obtained from the respectively named arguments to the tactic -/
+macro "init_next_block" h_run:ident blocki_eq:ident sn:ident block_size:num steps_left:num : tactic =>
+  `(tactic|
+    (-- use `let` over `obtain` to prevent `.intro` goal tags
+     let ⟨$sn:ident, ⟨$blocki_eq:ident, h_run_new⟩⟩ :=
+      @run_oneblock _ _ $block_size:num $steps_left:num $h_run:ident
+     replace $h_run:ident := h_run_new
+     clear h_run_new
+    ))
+
+section blockiTac
+
+/-- Apply the relevant pre-generated block lemma to an expression
+  `blocki_eq : run ?n ?s = ?s'`
+to add a new local hypothesis in terms of `w` and `write_mem`
+  `h_block_s' : ?s' = w _ _ (w _ _ (... ?s))`
+-/
+def blockiTac (blockiEq : Expr) (hBlock : Name) : SymReaderM Unit := fun ctx =>
+  withMainContext' <|
+  withInfoTraceNode m!"blockiTac: {blockiEq}\n {ctx.runSteps?} {ctx.effects}" (tag := "blockiTac") <| do
+    let pc := (Nat.toDigits 16 ctx.pc.toNat).asString
+    --  ^^ The PC in hex
+    let blockiLemma := Name.str ctx.program s!"blocki_eq_0x{pc}"
+    let eff := ctx.effects
+    let hStepExpr ← mkEqTrans
+      (← mkEqSymm blockiEq)
+      (← mkAppM blockiLemma #[
+        eff.programProof,
+        (← eff.getField .PC).proof,
+        (← eff.getField .ERR).proof
+      ])
+
+    let goal ← getMainGoal
+    let ⟨_, goal⟩ ← goal.note hBlock hStepExpr
+    replaceMainGoal [goal]
+
+end blockiTac
+
+/--
+Symbolically simulate a single step, according the the symbolic simulation
+context `c`, returning the context for the next step in simulation. -/
+def sym_block1 (blockSize stepsLeft : Nat) : SymM Unit := do
+  /- `withCurrHeartbeats` sets the initial heartbeats to the current heartbeats,
+  effectively resetting our heartbeat budget back to the maximum. -/
+  withCurrHeartbeats <| do
+
+  let stateNumber ← getCurrentStateNumber
+  withTraceNode m!"(sym_block1): simulating block {stateNumber}" (tag:="sym_block1") <|
+  withMainContext' do
+    withInfoTraceNode "verbose context" (tag := "infoDump") <| do
+      traceSymContext
+      trace[Tactic.sym.info] "Goal state:\n {← getMainGoal}"
+
+    let blocki_eq := Lean.mkIdent (.mkSimple s!"blocki_{← getCurrentStateName}")
+    let h_block   := Lean.mkIdent (.mkSimple s!"h_block_{stateNumber + blockSize}")
+
+    -- unfoldRun (fun _ => evalTacticAndTrace whileTac)
+
+    -- Add new state to local context
+    withTraceNode "initNextBlock" (tag := "initNextBlock") <| do
+      let hRunId      := mkIdent <|← getHRunName
+      let nextStateId := mkIdent <|← getNextStateName blockSize
+      let block_size : TSyntax `num := quote blockSize
+      let steps_left : TSyntax `num := quote stepsLeft
+      evalTacticAndTrace <|← `(tactic|
+        init_next_block $hRunId:ident $blocki_eq:ident $nextStateId:ident $block_size:num $steps_left:num
+      )
+
+    -- Apply relevant pre-generated `blocki` lemma
+    withMainContext' <| do
+      let blockiEq ← SymContext.findFromUserName blocki_eq.getId
+      blockiTac blockiEq.toExpr h_block.getId
+
+    -- WORKAROUND: eventually we'd like to eagerly simp away `if`s in the
+    -- pre-generation of instruction semantics. For now, though, we keep a
+    -- `simp` here
+    withMainContext' <| do
+      let hStep ← SymContext.findFromUserName h_block.getId
+
+      -- If we know SP is aligned, `simp` with that fact
+      if let some hSp := (← getThe AxEffects).stackAlignmentProof? then
+        let msg := m!"simplifying {hStep.toExpr} with {hSp}"
+        withTraceNode msg (tag := "simplifyHStep") <| do
+          let some goal ← do
+              let (ctx, simprocs) ← LNSymSimpContext
+                (config := {decide := false}) (exprs := #[hSp])
+              let goal ← getMainGoal
+              LNSymSimp goal ctx simprocs hStep.fvarId
+            | throwError "internal error: simp closed goal unexpectedly"
+          replaceMainGoal [goal]
+      else
+        trace[Tactic.sym.info] "we have no relevant local hypotheses, \
+          skipping simplification step"
+
+    -- Prepare `h_program`,`h_err`,`h_pc`, etc. for next state
+    withMainContext' <| do
+      let hBlock ← SymContext.findFromUserName h_block.getId
+      -- ^^ we can't reuse `hBlock` from before, since its fvarId might've been
+      --    changed by `simp`
+      explodeStep hBlock.toExpr blockSize
+      prepareForNextStep blockSize
+
+      let goal ← getMainGoal
+      let goal ← goal.clear hBlock.fvarId
+      replaceMainGoal [goal]
+      trace[Tactic.sym.info] "CurrentStateNumber: {← getCurrentStateNumber}"
+      trace[Tactic.sym.info] "CurrentState: {← getCurrentState}"
+      trace[Tactic.sym.info] "CurrentStateName: {← getCurrentStateName}"
+      traceHeartbeats
+
+syntax sym_block_size := "(" "block_size" " := " num ")"
+syntax sym_block_sizes := "(" "block_sizes" " := " "[" num,* "]" ")"
+
+/--
+Get the first `n` elements of the list `xs`, where `acc` is the accumulator.
+
+(FIXME) Implicit assumption: `xs` has at least one assumption.
+-/
+def first_n (n : Nat) (xs acc : List Nat) : List Nat :=
+  match n with
+  | 0 => acc.reverse
+  | n' + 1 => first_n n' xs.tail (List.headD xs 0 :: acc)
+
+/-- info: 5 -/
+#guard_msgs in
+#eval (first_n 1 [5, 2, 2, 1] []).foldl Nat.add 0
+
+open Elab.Term (elabTerm) in
+elab "sym_block" n:num
+                 -- block_size:(sym_block_size)?
+                 block_sizes:(sym_block_sizes)?
+                 s:(sym_at)? : tactic => do
+  traceHeartbeats "initial heartbeats"
+
+  let s ← s.mapM fun
+    | `(sym_at|at $s:ident) => pure s.getId
+    | _ => Lean.Elab.throwUnsupportedSyntax
+  let block_sizes ← block_sizes.mapM (fun
+  | `(sym_block_sizes|(block_sizes := [$elems,*])) => do
+      let size_exprs ← elems.getElems.mapM (fun elem => do
+        let size := elem.getNat
+        return (mkNatLit size))
+      let size_terms ← size_exprs.mapM (fun e => do
+          let some val ← Lean.Meta.getNatValue? e | throwError ""
+          return val)
+      dbg_trace s!"size_terms: {size_terms}"
+      pure size_terms.toList
+  |  _ =>
+      -- (FIXME)
+      -- If no block size is specified, we step one instruction at a time.
+      pure [1])
+  let block_sizes := block_sizes.get!
+  trace[Tactic.sym.info] "block_sizes: {block_sizes}"
+
+  -- let block_size ← block_size.mapM (fun
+  -- | `(sym_block_size|(block_size := $val)) => pure val.getNat
+  -- |  _ => -- If no block size is specified, we step one instruction at a time.
+  --         pure 1)
+  -- let block_size := block_size.get!
+
+  let c ← SymContext.fromMainContext s
+  -- TODO: Is this `get!` safe?
+  -- let total_steps := c.runSteps?.get!
+  -- The number of instructions, not blocks, the user asked to simulate.
+  let sim_steps := n.getNat
+  -- We compute the number of blocks to be simulated using a ceiling divide.
+  -- Note that the last block can be < `block_size`.
+  -- let num_blocks := (sim_steps + block_size - 1) / block_size
+
+  SymM.run' c <| withMainContext' <|  do
+    -- Check pre-conditions
+    -- TODO
+    -- assertStepTheoremsGenerated
+    -- let n ← ensureAtMostRunSteps n.getNat
+
+    withMainContext' <| do
+      -- The main loop
+      -- for i in List.range num_blocks do
+      --   let block_size' := min (sim_steps - (i * block_size)) block_size
+      --   let steps_left := (total_steps - (i * block_size) - block_size')
+      --   sym_block1 block_size' steps_left
+      let mut ctr := 0
+      for bsize in block_sizes do
+        ctr := ctr + 1
+        let steps_left := sim_steps - ((first_n ctr block_sizes []).foldl Nat.add 0)
+        sym_block1 bsize steps_left
+
+    traceHeartbeats "symbolic simulation total"
+    withCurrHeartbeats <|
+    withTraceNode "Post processing" (tag := "postProccessing") <| do
+      let c ← getThe SymContext
+      -- Check if we can substitute the final state
+      if c.runSteps? = some 0 then
+        let msg := do
+          let hRun ← userNameToMessageData c.h_run
+          pure m!"runSteps := 0, substituting along {hRun}"
+        withMainContext' <|
+        withTraceNode `Tactic.sym (fun _ => msg) <| do
+          let sfEq ← mkEq (← getCurrentState) c.finalState
+
+          let goal ← getMainGoal
+          trace[Tactic.sym.info] "original goal:\n{goal}"
+          let ⟨hEqId, goal⟩ ← do
+            let hRun ← SymContext.findFromUserName c.h_run
+            goal.note `this (← mkEqSymm hRun.toExpr) sfEq
+          goal.withContext <| do
+            trace[Tactic.sym.info] "added {← userNameToMessageData `this} of type \
+              {sfEq} in:\n{goal}"
+
+          let goal ← subst goal hEqId
+          trace[Tactic.sym.info] "performed subsitutition in:\n{goal}"
+          replaceMainGoal [goal]
+
+      -- Rudimentary aggregation: we feed all the axiomatic effect hypotheses
+      -- added while symbolically evaluating to `simp`
+      withMainContext' <|
+      withTraceNode m!"aggregating (non-)effects" (tag := "aggregateEffects") <| do
+        let goal? ← LNSymSimp (← getMainGoal) c.aggregateSimpCtx c.aggregateSimprocs
+        replaceMainGoal goal?.toList
+
+      traceHeartbeats "aggregation"
